rocq/RocqOfSolidityTests/semanticTests/experimental/type_class/GeneratedTest.v
@@ -25,14 +25,17 @@ Module Constructor.
   Definition initial_state : State.t :=
     let address := environment.(Environment.address) in
     let account := {|
-      Account.balance := environment.(Environment.callvalue);
+      Account.balance := 0;
       Account.nonce := 1;
       Account.code := constructor_code.(Code.hex_name);
       Account.codedata := Memory.hex_string_as_bytes "";
       Account.storage := Memory.empty;
       Account.immutables := [];
     |} in
-    State.init <| State.accounts := [(address, account)] |>.
+    State.init
+      <| State.accounts := [(address, account)] |>
+      <| State.block_number := 1 |>
+      <| State.block_timestamp := 15 |>.
 
   Definition result_state :=
     eval_with_revert 5000 codes environment constructor_code.(Code.body) initial_state.
@@ -51,3 +54,35 @@ Definition final_state : State.t :=
     eval 5000 codes environment (update_current_code_for_deploy deployed_code.(Code.hex_name)) state
   ).
 End Constructor.
+
+(* // () -> 1, 0 *)
+Module Step1.
+  Definition environment : Environment.t :={|
+    Environment.caller := 0x1212121212121212121212121212120000000012;
+    Environment.callvalue := 0;
+    Environment.calldata := Memory.hex_string_as_bytes "";
+    Environment.address := 0xc06afe3a8444fc0004668591e8306bfb9968e79e;
+    Environment.code_name := deployed_code.(Code.hex_name);
+  |}.
+
+  Definition initial_state : State.t :=
+    State.init
+      <| State.accounts := Constructor.final_state.(State.accounts) |>
+      <| State.block_number := 2 |>
+      <| State.block_timestamp := 30 |>.
+
+  Definition result_state :=
+    eval_with_revert 5000 codes environment deployed_code.(Code.body) initial_state.
+
+  Definition result := fst result_state.
+  Definition state := snd result_state.
+
+  Definition expected_output : list Z :=
+    Memory.hex_string_as_bytes "00000000000000000000000000000000000000000000000000000000000000010000000000000000000000000000000000000000000000000000000000000000".
+
+  Goal Test.extract_output result state Test.Status.Success = inl expected_output.
+  Proof.
+    vm_compute.
+    reflexivity.
+  Qed.
+End Step1.
