rocq/RocqOfSolidityTests/semanticTests/events/events_with_same_name_inherited_emit/GeneratedTest.v
@@ -27,14 +27,17 @@ Module Constructor.
   Definition initial_state : State.t :=
     let address := environment.(Environment.address) in
     let account := {|
-      Account.balance := environment.(Environment.callvalue);
+      Account.balance := 0;
       Account.nonce := 1;
       Account.code := constructor_code.(Code.hex_name);
       Account.codedata := Memory.hex_string_as_bytes "";
       Account.storage := Memory.empty;
       Account.immutables := [];
     |} in
-    State.init <| State.accounts := [(address, account)] |>.
+    State.init
+      <| State.accounts := [(address, account)] |>
+      <| State.block_number := 1 |>
+      <| State.block_timestamp := 15 |>.
 
   Definition result_state :=
     eval_with_revert 5000 codes environment constructor_code.(Code.body) initial_state.
@@ -66,7 +69,10 @@ Module Step1.
   |}.
 
   Definition initial_state : State.t :=
-    State.init <| State.accounts := Constructor.final_state.(State.accounts) |>.
+    State.init
+      <| State.accounts := Constructor.final_state.(State.accounts) |>
+      <| State.block_number := 2 |>
+      <| State.block_timestamp := 30 |>.
 
   Definition result_state :=
     eval_with_revert 5000 codes environment deployed_code.(Code.body) initial_state.
@@ -96,7 +102,10 @@ Module Step2.
   |}.
 
   Definition initial_state : State.t :=
-    State.init <| State.accounts := Step1.state.(State.accounts) |>.
+    State.init
+      <| State.accounts := Step1.state.(State.accounts) |>
+      <| State.block_number := 3 |>
+      <| State.block_timestamp := 45 |>.
 
   Definition result_state :=
     eval_with_revert 5000 codes environment deployed_code.(Code.body) initial_state.
@@ -126,7 +135,10 @@ Module Step3.
   |}.
 
   Definition initial_state : State.t :=
-    State.init <| State.accounts := Step2.state.(State.accounts) |>.
+    State.init
+      <| State.accounts := Step2.state.(State.accounts) |>
+      <| State.block_number := 4 |>
+      <| State.block_timestamp := 60 |>.
 
   Definition result_state :=
     eval_with_revert 5000 codes environment deployed_code.(Code.body) initial_state.
