rocq/RocqOfSolidityTests/semanticTests/libraries/mapping_returns_in_library/GeneratedTest.v
@@ -26,14 +26,17 @@ Module Constructor.
   Definition initial_state : State.t :=
     let address := environment.(Environment.address) in
     let account := {|
-      Account.balance := environment.(Environment.callvalue);
+      Account.balance := 0;
       Account.nonce := 1;
       Account.code := constructor_code.(Code.hex_name);
       Account.codedata := Memory.hex_string_as_bytes "";
       Account.storage := Memory.empty;
       Account.immutables := [];
     |} in
-    State.init <| State.accounts := [(address, account)] |>.
+    State.init
+      <| State.accounts := [(address, account)] |>
+      <| State.block_number := 2 |>
+      <| State.block_timestamp := 30 |>.
 
   Definition result_state :=
     eval_with_revert 5000 codes environment constructor_code.(Code.body) initial_state.
@@ -64,7 +67,10 @@ Module Step1.
   |}.
 
   Definition initial_state : State.t :=
-    State.init <| State.accounts := Constructor.final_state.(State.accounts) |>.
+    State.init
+      <| State.accounts := Constructor.final_state.(State.accounts) |>
+      <| State.block_number := 3 |>
+      <| State.block_timestamp := 45 |>.
 
   Definition result_state :=
     eval_with_revert 5000 codes environment deployed_code.(Code.body) initial_state.
@@ -93,7 +99,10 @@ Module Step2.
   |}.
 
   Definition initial_state : State.t :=
-    State.init <| State.accounts := Step1.state.(State.accounts) |>.
+    State.init
+      <| State.accounts := Step1.state.(State.accounts) |>
+      <| State.block_number := 4 |>
+      <| State.block_timestamp := 60 |>.
 
   Definition result_state :=
     eval_with_revert 5000 codes environment deployed_code.(Code.body) initial_state.
@@ -122,7 +131,10 @@ Module Step3.
   |}.
 
   Definition initial_state : State.t :=
-    State.init <| State.accounts := Step2.state.(State.accounts) |>.
+    State.init
+      <| State.accounts := Step2.state.(State.accounts) |>
+      <| State.block_number := 5 |>
+      <| State.block_timestamp := 75 |>.
 
   Definition result_state :=
     eval_with_revert 5000 codes environment deployed_code.(Code.body) initial_state.
@@ -151,7 +163,10 @@ Module Step4.
   |}.
 
   Definition initial_state : State.t :=
-    State.init <| State.accounts := Step3.state.(State.accounts) |>.
+    State.init
+      <| State.accounts := Step3.state.(State.accounts) |>
+      <| State.block_number := 6 |>
+      <| State.block_timestamp := 90 |>.
 
   Definition result_state :=
     eval_with_revert 5000 codes environment deployed_code.(Code.body) initial_state.
@@ -180,7 +195,10 @@ Module Step5.
   |}.
 
   Definition initial_state : State.t :=
-    State.init <| State.accounts := Step4.state.(State.accounts) |>.
+    State.init
+      <| State.accounts := Step4.state.(State.accounts) |>
+      <| State.block_number := 7 |>
+      <| State.block_timestamp := 105 |>.
 
   Definition result_state :=
     eval_with_revert 5000 codes environment deployed_code.(Code.body) initial_state.
@@ -209,7 +227,10 @@ Module Step6.
   |}.
 
   Definition initial_state : State.t :=
-    State.init <| State.accounts := Step5.state.(State.accounts) |>.
+    State.init
+      <| State.accounts := Step5.state.(State.accounts) |>
+      <| State.block_number := 8 |>
+      <| State.block_timestamp := 120 |>.
 
   Definition result_state :=
     eval_with_revert 5000 codes environment deployed_code.(Code.body) initial_state.
@@ -238,7 +259,10 @@ Module Step7.
   |}.
 
   Definition initial_state : State.t :=
-    State.init <| State.accounts := Step6.state.(State.accounts) |>.
+    State.init
+      <| State.accounts := Step6.state.(State.accounts) |>
+      <| State.block_number := 9 |>
+      <| State.block_timestamp := 135 |>.
 
   Definition result_state :=
     eval_with_revert 5000 codes environment deployed_code.(Code.body) initial_state.
@@ -267,7 +291,10 @@ Module Step8.
   |}.
 
   Definition initial_state : State.t :=
-    State.init <| State.accounts := Step7.state.(State.accounts) |>.
+    State.init
+      <| State.accounts := Step7.state.(State.accounts) |>
+      <| State.block_number := 10 |>
+      <| State.block_timestamp := 150 |>.
 
   Definition result_state :=
     eval_with_revert 5000 codes environment deployed_code.(Code.body) initial_state.
@@ -296,7 +323,10 @@ Module Step9.
   |}.
 
   Definition initial_state : State.t :=
-    State.init <| State.accounts := Step8.state.(State.accounts) |>.
+    State.init
+      <| State.accounts := Step8.state.(State.accounts) |>
+      <| State.block_number := 11 |>
+      <| State.block_timestamp := 165 |>.
 
   Definition result_state :=
     eval_with_revert 5000 codes environment deployed_code.(Code.body) initial_state.
@@ -325,7 +355,10 @@ Module Step10.
   |}.
 
   Definition initial_state : State.t :=
-    State.init <| State.accounts := Step9.state.(State.accounts) |>.
+    State.init
+      <| State.accounts := Step9.state.(State.accounts) |>
+      <| State.block_number := 12 |>
+      <| State.block_timestamp := 180 |>.
 
   Definition result_state :=
     eval_with_revert 5000 codes environment deployed_code.(Code.body) initial_state.
@@ -354,7 +387,10 @@ Module Step11.
   |}.
 
   Definition initial_state : State.t :=
-    State.init <| State.accounts := Step10.state.(State.accounts) |>.
+    State.init
+      <| State.accounts := Step10.state.(State.accounts) |>
+      <| State.block_number := 13 |>
+      <| State.block_timestamp := 195 |>.
 
   Definition result_state :=
     eval_with_revert 5000 codes environment deployed_code.(Code.body) initial_state.
@@ -383,7 +419,10 @@ Module Step12.
   |}.
 
   Definition initial_state : State.t :=
-    State.init <| State.accounts := Step11.state.(State.accounts) |>.
+    State.init
+      <| State.accounts := Step11.state.(State.accounts) |>
+      <| State.block_number := 14 |>
+      <| State.block_timestamp := 210 |>.
 
   Definition result_state :=
     eval_with_revert 5000 codes environment deployed_code.(Code.body) initial_state.
@@ -412,7 +451,10 @@ Module Step13.
   |}.
 
   Definition initial_state : State.t :=
-    State.init <| State.accounts := Step12.state.(State.accounts) |>.
+    State.init
+      <| State.accounts := Step12.state.(State.accounts) |>
+      <| State.block_number := 15 |>
+      <| State.block_timestamp := 225 |>.
 
   Definition result_state :=
     eval_with_revert 5000 codes environment deployed_code.(Code.body) initial_state.
@@ -441,7 +483,10 @@ Module Step14.
   |}.
 
   Definition initial_state : State.t :=
-    State.init <| State.accounts := Step13.state.(State.accounts) |>.
+    State.init
+      <| State.accounts := Step13.state.(State.accounts) |>
+      <| State.block_number := 16 |>
+      <| State.block_timestamp := 240 |>.
 
   Definition result_state :=
     eval_with_revert 5000 codes environment deployed_code.(Code.body) initial_state.
@@ -470,7 +515,10 @@ Module Step15.
   |}.
 
   Definition initial_state : State.t :=
-    State.init <| State.accounts := Step14.state.(State.accounts) |>.
+    State.init
+      <| State.accounts := Step14.state.(State.accounts) |>
+      <| State.block_number := 17 |>
+      <| State.block_timestamp := 255 |>.
 
   Definition result_state :=
     eval_with_revert 5000 codes environment deployed_code.(Code.body) initial_state.
@@ -499,7 +547,10 @@ Module Step16.
   |}.
 
   Definition initial_state : State.t :=
-    State.init <| State.accounts := Step15.state.(State.accounts) |>.
+    State.init
+      <| State.accounts := Step15.state.(State.accounts) |>
+      <| State.block_number := 18 |>
+      <| State.block_timestamp := 270 |>.
 
   Definition result_state :=
     eval_with_revert 5000 codes environment deployed_code.(Code.body) initial_state.
@@ -528,7 +579,10 @@ Module Step17.
   |}.
 
   Definition initial_state : State.t :=
-    State.init <| State.accounts := Step16.state.(State.accounts) |>.
+    State.init
+      <| State.accounts := Step16.state.(State.accounts) |>
+      <| State.block_number := 19 |>
+      <| State.block_timestamp := 285 |>.
 
   Definition result_state :=
     eval_with_revert 5000 codes environment deployed_code.(Code.body) initial_state.
@@ -557,7 +611,10 @@ Module Step18.
   |}.
 
   Definition initial_state : State.t :=
-    State.init <| State.accounts := Step17.state.(State.accounts) |>.
+    State.init
+      <| State.accounts := Step17.state.(State.accounts) |>
+      <| State.block_number := 20 |>
+      <| State.block_timestamp := 300 |>.
 
   Definition result_state :=
     eval_with_revert 5000 codes environment deployed_code.(Code.body) initial_state.
@@ -586,7 +643,10 @@ Module Step19.
   |}.
 
   Definition initial_state : State.t :=
-    State.init <| State.accounts := Step18.state.(State.accounts) |>.
+    State.init
+      <| State.accounts := Step18.state.(State.accounts) |>
+      <| State.block_number := 21 |>
+      <| State.block_timestamp := 315 |>.
 
   Definition result_state :=
     eval_with_revert 5000 codes environment deployed_code.(Code.body) initial_state.
@@ -615,7 +675,10 @@ Module Step20.
   |}.
 
   Definition initial_state : State.t :=
-    State.init <| State.accounts := Step19.state.(State.accounts) |>.
+    State.init
+      <| State.accounts := Step19.state.(State.accounts) |>
+      <| State.block_number := 22 |>
+      <| State.block_timestamp := 330 |>.
 
   Definition result_state :=
     eval_with_revert 5000 codes environment deployed_code.(Code.body) initial_state.
@@ -644,7 +707,10 @@ Module Step21.
   |}.
 
   Definition initial_state : State.t :=
-    State.init <| State.accounts := Step20.state.(State.accounts) |>.
+    State.init
+      <| State.accounts := Step20.state.(State.accounts) |>
+      <| State.block_number := 23 |>
+      <| State.block_timestamp := 345 |>.
 
   Definition result_state :=
     eval_with_revert 5000 codes environment deployed_code.(Code.body) initial_state.
@@ -673,7 +739,10 @@ Module Step22.
   |}.
 
   Definition initial_state : State.t :=
-    State.init <| State.accounts := Step21.state.(State.accounts) |>.
+    State.init
+      <| State.accounts := Step21.state.(State.accounts) |>
+      <| State.block_number := 24 |>
+      <| State.block_timestamp := 360 |>.
 
   Definition result_state :=
     eval_with_revert 5000 codes environment deployed_code.(Code.body) initial_state.
@@ -702,7 +771,10 @@ Module Step23.
   |}.
 
   Definition initial_state : State.t :=
-    State.init <| State.accounts := Step22.state.(State.accounts) |>.
+    State.init
+      <| State.accounts := Step22.state.(State.accounts) |>
+      <| State.block_number := 25 |>
+      <| State.block_timestamp := 375 |>.
 
   Definition result_state :=
     eval_with_revert 5000 codes environment deployed_code.(Code.body) initial_state.
@@ -731,7 +803,10 @@ Module Step24.
   |}.
 
   Definition initial_state : State.t :=
-    State.init <| State.accounts := Step23.state.(State.accounts) |>.
+    State.init
+      <| State.accounts := Step23.state.(State.accounts) |>
+      <| State.block_number := 26 |>
+      <| State.block_timestamp := 390 |>.
 
   Definition result_state :=
     eval_with_revert 5000 codes environment deployed_code.(Code.body) initial_state.
@@ -760,7 +835,10 @@ Module Step25.
   |}.
 
   Definition initial_state : State.t :=
-    State.init <| State.accounts := Step24.state.(State.accounts) |>.
+    State.init
+      <| State.accounts := Step24.state.(State.accounts) |>
+      <| State.block_number := 27 |>
+      <| State.block_timestamp := 405 |>.
 
   Definition result_state :=
     eval_with_revert 5000 codes environment deployed_code.(Code.body) initial_state.
@@ -789,7 +867,10 @@ Module Step26.
   |}.
 
   Definition initial_state : State.t :=
-    State.init <| State.accounts := Step25.state.(State.accounts) |>.
+    State.init
+      <| State.accounts := Step25.state.(State.accounts) |>
+      <| State.block_number := 28 |>
+      <| State.block_timestamp := 420 |>.
 
   Definition result_state :=
     eval_with_revert 5000 codes environment deployed_code.(Code.body) initial_state.
@@ -818,7 +899,10 @@ Module Step27.
   |}.
 
   Definition initial_state : State.t :=
-    State.init <| State.accounts := Step26.state.(State.accounts) |>.
+    State.init
+      <| State.accounts := Step26.state.(State.accounts) |>
+      <| State.block_number := 29 |>
+      <| State.block_timestamp := 435 |>.
 
   Definition result_state :=
     eval_with_revert 5000 codes environment deployed_code.(Code.body) initial_state.
@@ -847,7 +931,10 @@ Module Step28.
   |}.
 
   Definition initial_state : State.t :=
-    State.init <| State.accounts := Step27.state.(State.accounts) |>.
+    State.init
+      <| State.accounts := Step27.state.(State.accounts) |>
+      <| State.block_number := 30 |>
+      <| State.block_timestamp := 450 |>.
 
   Definition result_state :=
     eval_with_revert 5000 codes environment deployed_code.(Code.body) initial_state.
@@ -876,7 +963,10 @@ Module Step29.
   |}.
 
   Definition initial_state : State.t :=
-    State.init <| State.accounts := Step28.state.(State.accounts) |>.
+    State.init
+      <| State.accounts := Step28.state.(State.accounts) |>
+      <| State.block_number := 31 |>
+      <| State.block_timestamp := 465 |>.
 
   Definition result_state :=
     eval_with_revert 5000 codes environment deployed_code.(Code.body) initial_state.
@@ -905,7 +995,10 @@ Module Step30.
   |}.
 
   Definition initial_state : State.t :=
-    State.init <| State.accounts := Step29.state.(State.accounts) |>.
+    State.init
+      <| State.accounts := Step29.state.(State.accounts) |>
+      <| State.block_number := 32 |>
+      <| State.block_timestamp := 480 |>.
 
   Definition result_state :=
     eval_with_revert 5000 codes environment deployed_code.(Code.body) initial_state.
@@ -934,7 +1027,10 @@ Module Step31.
   |}.
 
   Definition initial_state : State.t :=
-    State.init <| State.accounts := Step30.state.(State.accounts) |>.
+    State.init
+      <| State.accounts := Step30.state.(State.accounts) |>
+      <| State.block_number := 33 |>
+      <| State.block_timestamp := 495 |>.
 
   Definition result_state :=
     eval_with_revert 5000 codes environment deployed_code.(Code.body) initial_state.
@@ -963,7 +1059,10 @@ Module Step32.
   |}.
 
   Definition initial_state : State.t :=
-    State.init <| State.accounts := Step31.state.(State.accounts) |>.
+    State.init
+      <| State.accounts := Step31.state.(State.accounts) |>
+      <| State.block_number := 34 |>
+      <| State.block_timestamp := 510 |>.
 
   Definition result_state :=
     eval_with_revert 5000 codes environment deployed_code.(Code.body) initial_state.
@@ -992,7 +1091,10 @@ Module Step33.
   |}.
 
   Definition initial_state : State.t :=
-    State.init <| State.accounts := Step32.state.(State.accounts) |>.
+    State.init
+      <| State.accounts := Step32.state.(State.accounts) |>
+      <| State.block_number := 35 |>
+      <| State.block_timestamp := 525 |>.
 
   Definition result_state :=
     eval_with_revert 5000 codes environment deployed_code.(Code.body) initial_state.
@@ -1021,7 +1123,10 @@ Module Step34.
   |}.
 
   Definition initial_state : State.t :=
-    State.init <| State.accounts := Step33.state.(State.accounts) |>.
+    State.init
+      <| State.accounts := Step33.state.(State.accounts) |>
+      <| State.block_number := 36 |>
+      <| State.block_timestamp := 540 |>.
 
   Definition result_state :=
     eval_with_revert 5000 codes environment deployed_code.(Code.body) initial_state.
@@ -1050,7 +1155,10 @@ Module Step35.
   |}.
 
   Definition initial_state : State.t :=
-    State.init <| State.accounts := Step34.state.(State.accounts) |>.
+    State.init
+      <| State.accounts := Step34.state.(State.accounts) |>
+      <| State.block_number := 37 |>
+      <| State.block_timestamp := 555 |>.
 
   Definition result_state :=
     eval_with_revert 5000 codes environment deployed_code.(Code.body) initial_state.
@@ -1079,7 +1187,10 @@ Module Step36.
   |}.
 
   Definition initial_state : State.t :=
-    State.init <| State.accounts := Step35.state.(State.accounts) |>.
+    State.init
+      <| State.accounts := Step35.state.(State.accounts) |>
+      <| State.block_number := 38 |>
+      <| State.block_timestamp := 570 |>.
 
   Definition result_state :=
     eval_with_revert 5000 codes environment deployed_code.(Code.body) initial_state.
@@ -1108,7 +1219,10 @@ Module Step37.
   |}.
 
   Definition initial_state : State.t :=
-    State.init <| State.accounts := Step36.state.(State.accounts) |>.
+    State.init
+      <| State.accounts := Step36.state.(State.accounts) |>
+      <| State.block_number := 39 |>
+      <| State.block_timestamp := 585 |>.
 
   Definition result_state :=
     eval_with_revert 5000 codes environment deployed_code.(Code.body) initial_state.
@@ -1137,7 +1251,10 @@ Module Step38.
   |}.
 
   Definition initial_state : State.t :=
-    State.init <| State.accounts := Step37.state.(State.accounts) |>.
+    State.init
+      <| State.accounts := Step37.state.(State.accounts) |>
+      <| State.block_number := 40 |>
+      <| State.block_timestamp := 600 |>.
 
   Definition result_state :=
     eval_with_revert 5000 codes environment deployed_code.(Code.body) initial_state.
@@ -1166,7 +1283,10 @@ Module Step39.
   |}.
 
   Definition initial_state : State.t :=
-    State.init <| State.accounts := Step38.state.(State.accounts) |>.
+    State.init
+      <| State.accounts := Step38.state.(State.accounts) |>
+      <| State.block_number := 41 |>
+      <| State.block_timestamp := 615 |>.
 
   Definition result_state :=
     eval_with_revert 5000 codes environment deployed_code.(Code.body) initial_state.
@@ -1195,7 +1315,10 @@ Module Step40.
   |}.
 
   Definition initial_state : State.t :=
-    State.init <| State.accounts := Step39.state.(State.accounts) |>.
+    State.init
+      <| State.accounts := Step39.state.(State.accounts) |>
+      <| State.block_number := 42 |>
+      <| State.block_timestamp := 630 |>.
 
   Definition result_state :=
     eval_with_revert 5000 codes environment deployed_code.(Code.body) initial_state.
@@ -1224,7 +1347,10 @@ Module Step41.
   |}.
 
   Definition initial_state : State.t :=
-    State.init <| State.accounts := Step40.state.(State.accounts) |>.
+    State.init
+      <| State.accounts := Step40.state.(State.accounts) |>
+      <| State.block_number := 43 |>
+      <| State.block_timestamp := 645 |>.
 
   Definition result_state :=
     eval_with_revert 5000 codes environment deployed_code.(Code.body) initial_state.
@@ -1253,7 +1379,10 @@ Module Step42.
   |}.
 
   Definition initial_state : State.t :=
-    State.init <| State.accounts := Step41.state.(State.accounts) |>.
+    State.init
+      <| State.accounts := Step41.state.(State.accounts) |>
+      <| State.block_number := 44 |>
+      <| State.block_timestamp := 660 |>.
 
   Definition result_state :=
     eval_with_revert 5000 codes environment deployed_code.(Code.body) initial_state.
@@ -1282,7 +1411,10 @@ Module Step43.
   |}.
 
   Definition initial_state : State.t :=
-    State.init <| State.accounts := Step42.state.(State.accounts) |>.
+    State.init
+      <| State.accounts := Step42.state.(State.accounts) |>
+      <| State.block_number := 45 |>
+      <| State.block_timestamp := 675 |>.
 
   Definition result_state :=
     eval_with_revert 5000 codes environment deployed_code.(Code.body) initial_state.
@@ -1311,7 +1443,10 @@ Module Step44.
   |}.
 
   Definition initial_state : State.t :=
-    State.init <| State.accounts := Step43.state.(State.accounts) |>.
+    State.init
+      <| State.accounts := Step43.state.(State.accounts) |>
+      <| State.block_number := 46 |>
+      <| State.block_timestamp := 690 |>.
 
   Definition result_state :=
     eval_with_revert 5000 codes environment deployed_code.(Code.body) initial_state.
