rocq/RocqOfSolidityTests/semanticTests/storage/storage_boundary_struct_array_packed/GeneratedTest.v
@@ -25,14 +25,17 @@ Module Constructor.
   Definition initial_state : State.t :=
     let address := environment.(Environment.address) in
     let account := {|
-      Account.balance := environment.(Environment.callvalue);
+      Account.balance := 0;
       Account.nonce := 1;
       Account.code := constructor_code.(Code.hex_name);
       Account.codedata := Memory.hex_string_as_bytes "";
       Account.storage := Memory.empty;
       Account.immutables := [];
     |} in
-    State.init <| State.accounts := [(address, account)] |>.
+    State.init
+      <| State.accounts := [(address, account)] |>
+      <| State.block_number := 1 |>
+      <| State.block_timestamp := 15 |>.
 
   Definition result_state :=
     eval_with_revert 5000 codes environment constructor_code.(Code.body) initial_state.
@@ -63,7 +66,10 @@ Module Step1.
   |}.
 
   Definition initial_state : State.t :=
-    State.init <| State.accounts := Constructor.final_state.(State.accounts) |>.
+    State.init
+      <| State.accounts := Constructor.final_state.(State.accounts) |>
+      <| State.block_number := 2 |>
+      <| State.block_timestamp := 30 |>.
 
   Definition result_state :=
     eval_with_revert 5000 codes environment deployed_code.(Code.body) initial_state.
@@ -92,7 +98,10 @@ Module Step2.
   |}.
 
   Definition initial_state : State.t :=
-    State.init <| State.accounts := Step1.state.(State.accounts) |>.
+    State.init
+      <| State.accounts := Step1.state.(State.accounts) |>
+      <| State.block_number := 3 |>
+      <| State.block_timestamp := 45 |>.
 
   Definition result_state :=
     eval_with_revert 5000 codes environment deployed_code.(Code.body) initial_state.
@@ -121,7 +130,10 @@ Module Step3.
   |}.
 
   Definition initial_state : State.t :=
-    State.init <| State.accounts := Step2.state.(State.accounts) |>.
+    State.init
+      <| State.accounts := Step2.state.(State.accounts) |>
+      <| State.block_number := 4 |>
+      <| State.block_timestamp := 60 |>.
 
   Definition result_state :=
     eval_with_revert 5000 codes environment deployed_code.(Code.body) initial_state.
@@ -153,7 +165,10 @@ Module Step4.
   |}.
 
   Definition initial_state : State.t :=
-    State.init <| State.accounts := Step3.state.(State.accounts) |>.
+    State.init
+      <| State.accounts := Step3.state.(State.accounts) |>
+      <| State.block_number := 5 |>
+      <| State.block_timestamp := 75 |>.
 
   Definition result_state :=
     eval_with_revert 5000 codes environment deployed_code.(Code.body) initial_state.
@@ -182,7 +197,10 @@ Module Step5.
   |}.
 
   Definition initial_state : State.t :=
-    State.init <| State.accounts := Step4.state.(State.accounts) |>.
+    State.init
+      <| State.accounts := Step4.state.(State.accounts) |>
+      <| State.block_number := 6 |>
+      <| State.block_timestamp := 90 |>.
 
   Definition result_state :=
     eval_with_revert 5000 codes environment deployed_code.(Code.body) initial_state.
@@ -211,7 +229,10 @@ Module Step6.
   |}.
 
   Definition initial_state : State.t :=
-    State.init <| State.accounts := Step5.state.(State.accounts) |>.
+    State.init
+      <| State.accounts := Step5.state.(State.accounts) |>
+      <| State.block_number := 7 |>
+      <| State.block_timestamp := 105 |>.
 
   Definition result_state :=
     eval_with_revert 5000 codes environment deployed_code.(Code.body) initial_state.
@@ -240,7 +261,10 @@ Module Step7.
   |}.
 
   Definition initial_state : State.t :=
-    State.init <| State.accounts := Step6.state.(State.accounts) |>.
+    State.init
+      <| State.accounts := Step6.state.(State.accounts) |>
+      <| State.block_number := 8 |>
+      <| State.block_timestamp := 120 |>.
 
   Definition result_state :=
     eval_with_revert 5000 codes environment deployed_code.(Code.body) initial_state.
@@ -272,7 +296,10 @@ Module Step8.
   |}.
 
   Definition initial_state : State.t :=
-    State.init <| State.accounts := Step7.state.(State.accounts) |>.
+    State.init
+      <| State.accounts := Step7.state.(State.accounts) |>
+      <| State.block_number := 9 |>
+      <| State.block_timestamp := 135 |>.
 
   Definition result_state :=
     eval_with_revert 5000 codes environment deployed_code.(Code.body) initial_state.
@@ -301,7 +328,10 @@ Module Step9.
   |}.
 
   Definition initial_state : State.t :=
-    State.init <| State.accounts := Step8.state.(State.accounts) |>.
+    State.init
+      <| State.accounts := Step8.state.(State.accounts) |>
+      <| State.block_number := 10 |>
+      <| State.block_timestamp := 150 |>.
 
   Definition result_state :=
     eval_with_revert 5000 codes environment deployed_code.(Code.body) initial_state.
@@ -330,7 +360,10 @@ Module Step10.
   |}.
 
   Definition initial_state : State.t :=
-    State.init <| State.accounts := Step9.state.(State.accounts) |>.
+    State.init
+      <| State.accounts := Step9.state.(State.accounts) |>
+      <| State.block_number := 11 |>
+      <| State.block_timestamp := 165 |>.
 
   Definition result_state :=
     eval_with_revert 5000 codes environment deployed_code.(Code.body) initial_state.
@@ -359,7 +392,10 @@ Module Step11.
   |}.
 
   Definition initial_state : State.t :=
-    State.init <| State.accounts := Step10.state.(State.accounts) |>.
+    State.init
+      <| State.accounts := Step10.state.(State.accounts) |>
+      <| State.block_number := 12 |>
+      <| State.block_timestamp := 180 |>.
 
   Definition result_state :=
     eval_with_revert 5000 codes environment deployed_code.(Code.body) initial_state.
@@ -389,7 +425,10 @@ Module Step12.
   |}.
 
   Definition initial_state : State.t :=
-    State.init <| State.accounts := Step11.state.(State.accounts) |>.
+    State.init
+      <| State.accounts := Step11.state.(State.accounts) |>
+      <| State.block_number := 13 |>
+      <| State.block_timestamp := 195 |>.
 
   Definition result_state :=
     eval_with_revert 5000 codes environment deployed_code.(Code.body) initial_state.
@@ -418,7 +457,10 @@ Module Step13.
   |}.
 
   Definition initial_state : State.t :=
-    State.init <| State.accounts := Step12.state.(State.accounts) |>.
+    State.init
+      <| State.accounts := Step12.state.(State.accounts) |>
+      <| State.block_number := 14 |>
+      <| State.block_timestamp := 210 |>.
 
   Definition result_state :=
     eval_with_revert 5000 codes environment deployed_code.(Code.body) initial_state.
@@ -447,7 +489,10 @@ Module Step14.
   |}.
 
   Definition initial_state : State.t :=
-    State.init <| State.accounts := Step13.state.(State.accounts) |>.
+    State.init
+      <| State.accounts := Step13.state.(State.accounts) |>
+      <| State.block_number := 15 |>
+      <| State.block_timestamp := 225 |>.
 
   Definition result_state :=
     eval_with_revert 5000 codes environment deployed_code.(Code.body) initial_state.
@@ -477,7 +522,10 @@ Module Step15.
   |}.
 
   Definition initial_state : State.t :=
-    State.init <| State.accounts := Step14.state.(State.accounts) |>.
+    State.init
+      <| State.accounts := Step14.state.(State.accounts) |>
+      <| State.block_number := 16 |>
+      <| State.block_timestamp := 240 |>.
 
   Definition result_state :=
     eval_with_revert 5000 codes environment deployed_code.(Code.body) initial_state.
@@ -509,7 +557,10 @@ Module Step16.
   |}.
 
   Definition initial_state : State.t :=
-    State.init <| State.accounts := Step15.state.(State.accounts) |>.
+    State.init
+      <| State.accounts := Step15.state.(State.accounts) |>
+      <| State.block_number := 17 |>
+      <| State.block_timestamp := 255 |>.
 
   Definition result_state :=
     eval_with_revert 5000 codes environment deployed_code.(Code.body) initial_state.
@@ -538,7 +589,10 @@ Module Step17.
   |}.
 
   Definition initial_state : State.t :=
-    State.init <| State.accounts := Step16.state.(State.accounts) |>.
+    State.init
+      <| State.accounts := Step16.state.(State.accounts) |>
+      <| State.block_number := 18 |>
+      <| State.block_timestamp := 270 |>.
 
   Definition result_state :=
     eval_with_revert 5000 codes environment deployed_code.(Code.body) initial_state.
@@ -567,7 +621,10 @@ Module Step18.
   |}.
 
   Definition initial_state : State.t :=
-    State.init <| State.accounts := Step17.state.(State.accounts) |>.
+    State.init
+      <| State.accounts := Step17.state.(State.accounts) |>
+      <| State.block_number := 19 |>
+      <| State.block_timestamp := 285 |>.
 
   Definition result_state :=
     eval_with_revert 5000 codes environment deployed_code.(Code.body) initial_state.
@@ -596,7 +653,10 @@ Module Step19.
   |}.
 
   Definition initial_state : State.t :=
-    State.init <| State.accounts := Step18.state.(State.accounts) |>.
+    State.init
+      <| State.accounts := Step18.state.(State.accounts) |>
+      <| State.block_number := 20 |>
+      <| State.block_timestamp := 300 |>.
 
   Definition result_state :=
     eval_with_revert 5000 codes environment deployed_code.(Code.body) initial_state.
@@ -625,7 +685,10 @@ Module Step20.
   |}.
 
   Definition initial_state : State.t :=
-    State.init <| State.accounts := Step19.state.(State.accounts) |>.
+    State.init
+      <| State.accounts := Step19.state.(State.accounts) |>
+      <| State.block_number := 21 |>
+      <| State.block_timestamp := 315 |>.
 
   Definition result_state :=
     eval_with_revert 5000 codes environment deployed_code.(Code.body) initial_state.
@@ -654,7 +717,10 @@ Module Step21.
   |}.
 
   Definition initial_state : State.t :=
-    State.init <| State.accounts := Step20.state.(State.accounts) |>.
+    State.init
+      <| State.accounts := Step20.state.(State.accounts) |>
+      <| State.block_number := 22 |>
+      <| State.block_timestamp := 330 |>.
 
   Definition result_state :=
     eval_with_revert 5000 codes environment deployed_code.(Code.body) initial_state.
@@ -683,7 +749,10 @@ Module Step22.
   |}.
 
   Definition initial_state : State.t :=
-    State.init <| State.accounts := Step21.state.(State.accounts) |>.
+    State.init
+      <| State.accounts := Step21.state.(State.accounts) |>
+      <| State.block_number := 23 |>
+      <| State.block_timestamp := 345 |>.
 
   Definition result_state :=
     eval_with_revert 5000 codes environment deployed_code.(Code.body) initial_state.
@@ -712,7 +781,10 @@ Module Step23.
   |}.
 
   Definition initial_state : State.t :=
-    State.init <| State.accounts := Step22.state.(State.accounts) |>.
+    State.init
+      <| State.accounts := Step22.state.(State.accounts) |>
+      <| State.block_number := 24 |>
+      <| State.block_timestamp := 360 |>.
 
   Definition result_state :=
     eval_with_revert 5000 codes environment deployed_code.(Code.body) initial_state.
